---
layout: post
title:  "常用数学公式"
date:   2017-04-28 15：08:09 -0800
categories: math
tags: math latex
---

x=\frac{-b\pm\sqrt{b^2-4ac}}{2a}

$$x=\frac{-b\pm\sqrt{b^2-4ac}}{2a}$$

\sum_{i=1}^{n}\dfrac{ 1 } {n!} = e

$$  \sum_{i=1}^{n}\dfrac{ 1 } {n!} = e$$ 

e^x  = 1+ x+ \dfrac{x^2}{2!}+.......\dfrac{x^n}{n!}

$$ e^x  = 1+ x+ \dfrac{x^2}{2!}+.......\dfrac{x^n}{n!}$$


e^1 = e = 1+ \dfrac{1}{2!}+ 
x =1

$$ e^1 = e = 1+ \dfrac{1}{2!}+ $$

f(x) = f(x_0)+f'(x_0)(x-x_0)+\dfrac{f''(x_0)}{2!}(x-x_0)^2+.........+\dfrac{f^n(x_0)}{n!}(x-x_0)^n

$$ f(x) = f(x_0)+f'(x_0)(x-x_0)+\dfrac{f''(x_0)}{2!}(x-x_0)^2+.........+\dfrac{f^n(x_0)}{n!}(x-x_0)^n$$

x = \dfrac{-b \pm \sqrt{b^2 - 4ac}}{2a}

$$	x = \dfrac{-b \pm \sqrt{b^2 - 4ac}}{2a} $$











